Progress on relaxing wait_time bounds

pancake/proofs/time_to_panProofScript.sml
@@ -574,7 +574,7 @@ Definition wait_time_locals_def:
   wait_time_locals (:α) fm swt ffi =
   ∃wt st.
     FLOOKUP fm «wakeUpAt» = SOME (ValWord (n2w (wt + st))) ∧
-    wt + st < dimword (:α) ∧
+    (* wt + st < dimword (:α) ∧ *)
     case swt of
     | NONE => T
     | SOME swt =>
@@ -910,6 +910,18 @@ Definition ffi_rels_after_init_def:
                 ffi := ffi_call_ffi (:α) t.be t.ffi bytes|>)
 End
 
+
+Definition sum_delays_def:
+  sum_delays (:α) lbls (ffi:time_input) ⇔
+    SUM (MAP (λlbl.
+               case lbl of
+               | LDelay d => d
+               | _ => 0) lbls) + FST (ffi 0) = dimword (:α) − 2 ∧
+    (∀n.
+       FST (ffi n) = dimword (:α) − 2 ⇒
+       ffi (n+1) = (dimword (:α) − 1, 0) ∧
+       mem_read_ffi_results (:α) ffi (n+1))
+End
 
 Theorem length_get_bytes:
   ∀w be.
@@ -5686,13 +5698,14 @@ Theorem step_input:
         SOME (ValWord (n2w (
           case s'.waitTime of
           | NONE => 1
-          | _ => 0))) ∧
+          | _ => 0))) (* ∧
       (case s'.waitTime of
        | SOME wt => FST (t.ffi.ffi_state 0) + wt < dimword (:α)
-       | _ => T)
+       | _ => T) *)
 
 Proof
-  rw [] >>
+  cheat
+  (*rw [] >>
   fs [task_controller_def] >>
   fs [panLangTheory.nested_seq_def] >>
   qmatch_goalsub_abbrev_tac ‘evaluate (Seq _ q, _)’ >>
@@ -6524,7 +6537,7 @@ Proof
   gs [DROP_LENGTH_APPEND, decode_io_events_def, io_events_dest_def,
       mk_ti_event_def, decode_io_event_def]  >>
   cases_on ‘ t.ffi.ffi_state 1’ >> gs [] >>
-  gs [to_input_def]
+  gs [to_input_def] *)
 QED
 
 
@@ -6565,12 +6578,13 @@ Theorem step_output:
         SOME (ValWord (n2w (
           case s'.waitTime of
           | NONE => 1
-          | _ => 0))) ∧
+          | _ => 0))) (* ∧
       (case s'.waitTime of
        | SOME wt => FST (t.ffi.ffi_state 0) + wt < dimword (:α)
-       | _ => T)
+       | _ => T) *)
 Proof
-  rw [] >>
+  cheat
+  (* rw [] >>
   fs [] >>
   fs [step_cases, task_controller_def,
       panLangTheory.nested_seq_def] >>
@@ -7172,9 +7186,11 @@ Proof
     rw [] >>
     qexists_tac ‘#"g"’ >> gs []) >>
   gs [mlintTheory.num_to_str_thm, toString_toNum_cancel]
+  *)
 QED
 
 
+(*
 Theorem step_delay_until_max:
   ∀prog n s (t:('a,time_input) panSem$state) cycles.
     step prog (LDelay (dimword (:α) − (n + 2))) (dimword (:α) − 1) n s
@@ -7364,8 +7380,7 @@ Proof
   gs [ffi_call_ffi_def, state_component_equality] >>
   gs [delay_io_events_rel_def]
 QED
-
-
+*)
 
 Theorem steps_sts_length_eq_lbls:
   ∀lbls prog m n st sts.
@@ -7426,6 +7441,9 @@ Proof
     gs [] >>
     conj_asm1_tac
     >- (
+      (*
+      wait_time_locals (:α) t.locals st.waitTime t.ffi.ffi_state
+      *)
       gs [wait_time_locals_def] >>
       qexists_tac ‘wt’ >>
       qexists_tac ‘st'’ >>
@@ -7435,19 +7453,25 @@ Proof
       gs [step_cases] >>
       rveq >> gs [] >>
       fs [mkState_def] >>
-      cases_on ‘n < x’
-      >- (
-        fs [wakeup_rel_def] >>
-        fs [nexts_ffi_def] >>
-        ‘(st' + wt) MOD dimword (:α) = st' + wt’ by (
-          match_mp_tac LESS_MOD >>
-          gs []) >>
-        ‘(x + FST (t.ffi.ffi_state 0)) MOD dimword (:α) =
-         x + FST (t.ffi.ffi_state 0)’ by (
-          match_mp_tac LESS_MOD >>
-          gs [timeSemTheory.step_cases]) >>
-        gs [delay_rep_def]) >>
-      gs []) >>
+      strip_tac >>
+      reverse (cases_on ‘n < x’)
+      >- gs [] >>
+
+      fs [wakeup_rel_def] >>
+      fs [nexts_ffi_def] >>
+      cases_on ‘’ >>
+
+      ‘(st' + wt) MOD dimword (:α) = st' + wt’ by (
+        match_mp_tac LESS_MOD >>
+        gs []) >>
+      ‘(x + FST (t.ffi.ffi_state 0)) MOD dimword (:α) =
+       x + FST (t.ffi.ffi_state 0)’ by (
+        match_mp_tac LESS_MOD >>
+        gs [timeSemTheory.step_cases]) >>
+      gs [delay_rep_def]) >>
+
+
+
     conj_asm1_tac
     >- (
       gs [delay_io_events_rel_def] >>
@@ -7581,18 +7605,6 @@ Proof
   gs []
 QED
 
-Definition sum_delays_def:
-  sum_delays (:α) lbls (ffi:time_input) ⇔
-    SUM (MAP (λlbl.
-               case lbl of
-               | LDelay d => d
-               | _ => 0) lbls) + FST (ffi 0) = dimword (:α) − 2 ∧
-    (∀n.
-       FST (ffi n) = dimword (:α) − 2 ⇒
-       ffi (n+1) = (dimword (:α) − 1, 0) ∧
-       mem_read_ffi_results (:α) ffi (n+1))
-End
-
 Theorem steps_io_event_thm:
   ∀labels prog n st sts (t:('a,time_input) panSem$state).
     steps prog labels (dimword (:α) - 1) n st sts ∧
@@ -7641,12 +7653,29 @@ Proof
     ‘FLOOKUP t.locals «isInput» = SOME (ValWord 1w)’ by
       gs [assumptions_def, event_inv_def] >>
     ‘∃w. eval t wait = SOME (ValWord w) ∧ w ≠ 0w’ by (
-      ‘FLOOKUP t.locals «waitSet» = SOME (ValWord 1w)’ by
-         gs [assumptions_def, state_rel_def, equivs_def, active_low_def] >>
-      drule step_delay_eval_wait_not_zero >>
+      cases_on ‘st.waitTime’
+      >- (
+        ‘FLOOKUP t.locals «waitSet» = SOME (ValWord 1w)’ by
+           gs [assumptions_def, state_rel_def, equivs_def, active_low_def] >>
+        drule step_delay_eval_wait_not_zero >>
+        impl_tac
+        >- gs [assumptions_def, state_rel_def, mkState_def,
+               equivs_def, time_vars_def, active_low_def] >>
+        gs []) >>
+      gs [] >>
+      ‘FLOOKUP t.locals «waitSet» = SOME (ValWord 0w)’ by
+        gs [assumptions_def, state_rel_def, equivs_def, active_low_def] >>
+      drule step_wait_delay_eval_wait_not_zero >>
       impl_tac
-      >- gs [assumptions_def, state_rel_def, mkState_def,
-             equivs_def, time_vars_def, active_low_def] >>
+      >- (
+        conj_tac >- gs [] >>
+        gs [assumptions_def, state_rel_def] >>
+        pairarg_tac >> gs [] >>
+        qexists_tac ‘dimword (:α) − 2’ >>
+        gs [] >>
+        gs [wait_time_locals_def] >>
+        qexists_tac ‘st' + wt’ >>
+        gs []) >>
       gs []) >>
     gs [eval_upd_clock_eq] >>
     pairarg_tac >> fs [] >>
